Fifteen/Data/Board/Cycle.lean
@@ -1,0 +1,192 @@
+/-
+Copyright (c) 2023 Jun Yoshida. All rights reserved.
+Released under Apache 2.0 license as described in the file LICENSE.
+-/
+
+import Fifteen.Data.Fin.Basic
+import Fifteen.Data.Board.Basic
+
+/-!
+# Basic cyclic moves
+-/
+
+-- Disable auto-binding of unbounded variables
+set_option autoImplicit false
+
+
+namespace Board
+
+variable {m n : Nat}
+
+protected def pivot (i : Fin m) (j : Fin n) : Fin ((m+1)*(n+1)) :=
+  Fin.rlexProd i.castSucc j.castSucc
+
+theorem pivot_lt_last (i : Fin m) (j : Fin n) : (Board.pivot i j).1 < (m+1)*(n+1)-1 := by
+  conv =>
+    rhs; change (m+1)*n + m; rw [Nat.add_comm _ m]
+    change (Fin.rlexProd (Fin.last m) (Fin.last n)).1
+  exact Fin.rlexProd_lt_of_snd _ _ j.2
+
+protected def pathL (i : Fin m) (j : Fin n) : List (Fin ((m+1)*(n+1))) :=
+  List.ofFn fun (k : Fin (n-j.1)) =>
+    Fin.rlexProd i.castSucc <| (k.natAdd j.1).succ.castLE <| by
+      rewrite [Nat.add_sub_cancel' (Nat.le_of_lt j.2)]
+      exact .refl
+
+theorem lt_last_of_mem_pathL (i : Fin m) (j : Fin n) (a : Fin ((m+1)*(n+1))) (ha : a ∈ Board.pathL i j) : a.1 < (m+1)*(n+1)-1 := by
+  conv at ha => dsimp [Board.pathL]; rw [List.mem_ofFn]
+  have ⟨⟨k,hk⟩,ha⟩ := ha; cases ha; dsimp
+  conv =>
+    change (i.1 + (m+1)*(j.1+k+1)).succ ≤ (m+1)*n+m
+    rw [← Nat.succ_add i.1, Nat.add_comm _ m]
+  refine Nat.add_le_add i.2 ?_
+  refine Nat.mul_le_mul_left (m+1) ?_
+  rewrite [Nat.add_comm j.1 k]
+  exact Nat.add_lt_of_lt_sub hk
+
+theorem pivot_not_mem_pathL (i : Fin m) (j : Fin n) : Board.pivot i j ∉ Board.pathL i j := by
+  dsimp [Board.pathL]; simp only [List.mem_ofFn, not_exists]
+  intro k
+  refine Fin.ne_of_val_ne (Nat.ne_of_gt ?_)
+  apply Fin.rlexProd_lt_of_snd
+  show j.1 < j.1 + k + 1
+  rewrite [Nat.add_assoc]
+  exact j.1.lt_add_of_pos_right k.1.zero_lt_succ
+
+variable (n) in
+protected def pathB (i : Fin m) : List (Fin ((m+1)*(n+1))) :=
+  List.ofFn fun (k : Fin (m-i.1-1)) =>
+    Fin.rlexProd
+      ((i.eadd k).succ.castLT <| by
+        rewrite [Fin.val_succ, Fin.val_eadd, Nat.add_comm i.1 k.1, Nat.add_assoc]
+        apply Nat.add_lt_of_lt_sub
+        rewrite [Nat.succ_sub_succ]
+        exact trans k.2 ((m-i.1).sub_le 1)
+      )
+      (Fin.last n)
+
+variable (n) in
+theorem lt_last_of_mem_pathB (i : Fin m) (a : Fin ((m+1)*(n+1))) (ha : a ∈ Board.pathB n i) : a.1 < (m+1)*(n+1)-1 := by
+  conv at ha => dsimp [Board.pathB]; rw [List.mem_ofFn]
+  have ⟨⟨k,hk⟩,ha⟩ := ha; cases ha; simp
+  conv => rhs; change (m+1)*n + m; rw [Nat.add_comm _ m]
+  refine Nat.add_lt_add_right ?_ _
+  rewrite [Nat.add_comm i.1 k, Nat.add_assoc]
+  exact Nat.add_lt_of_lt_sub hk
+
+theorem pivot_not_mem_pathB (i : Fin m) (j : Fin n) : Board.pivot i j ∉ Board.pathB n i := by
+  dsimp [Board.pathB]; simp only [List.mem_ofFn, not_exists]
+  intro k
+  refine Fin.ne_of_val_ne (Nat.ne_of_gt ?_)
+  exact Fin.rlexProd_lt_of_snd _ _ j.2
+
+variable (m) in
+protected def pathR (j : Fin n) : List (Fin ((m+1)*(n+1))) :=
+  List.ofFn fun (⟨k,_⟩ : Fin (n-j.1)) =>
+    Fin.rlexProd (Fin.last m) <| .mk (n-k-1) <| by
+      rewrite [← Nat.sub_add_eq]
+      exact trans (n.sub_le (k+1)) n.lt_succ_self
+
+variable (m) in
+theorem lt_last_of_mem_pathR (j : Fin n) (a : Fin ((m+1)*(n+1))) (ha : a ∈ Board.pathR m j) : a.1 < (m+1)*(n+1)-1 := by
+  conv at ha => dsimp [Board.pathR]; rw [List.mem_ofFn]
+  have ⟨⟨k,hk⟩,ha⟩ := ha; cases ha; simp
+  conv => rhs; change (m+1)*n + m; rw [Nat.add_comm _ m]
+  refine Nat.add_lt_add_left ?_ m
+  refine Nat.mul_lt_mul_of_pos_left ?_ m.zero_lt_succ
+  rewrite [← Nat.sub_add_eq]
+  exact n.sub_lt j.pos k.zero_lt_succ
+
+theorem pivot_not_mem_pathR (i : Fin m) (j : Fin n) : Board.pivot i j ∉ Board.pathR m j := by
+  dsimp [Board.pathR, Board.pivot]; simp only [List.mem_ofFn, not_exists]
+  intro k
+  refine Fin.ne_of_val_ne (Nat.ne_of_gt ?_)
+  apply Fin.rlexProd_lt_iff.mpr
+  show j.1 < n - k.1 - 1 ∨ _ = _ ∧ i.1 < m
+  rewrite [Decidable.or_iff_not_imp_left]
+  simp only [Nat.not_lt, Fin.is_lt, and_true]
+  intro h
+  apply Fin.eq_of_val_eq; dsimp
+  apply Nat.le_antisymm ?_ h
+  rewrite [← Nat.sub_add_eq]
+  apply Nat.le_sub_of_add_le
+  show j.1 + k.1 < n
+  rewrite [Nat.add_comm j.1 k.1]
+  exact Nat.add_lt_of_lt_sub k.2
+
+protected def pathT (i : Fin m) (j : Fin n) : List (Fin ((m+1)*(n+1))) :=
+  List.ofFn fun (⟨k,_⟩ : Fin (m-i.1-1)) =>
+    Fin.rlexProd
+      (.mk (m-k-1) <| by
+        rewrite [← Nat.sub_add_eq]
+        exact trans (m.sub_le (k+1)) m.lt_succ_self
+      )
+      j.castSucc
+
+theorem lt_last_of_mem_pathT (i : Fin m) (j : Fin n) (a : Fin ((m+1)*(n+1))) (ha : a ∈ Board.pathT i j) : a.1 < (m+1)*(n+1)-1 := by
+  conv at ha => dsimp [Board.pathT]; rw [List.mem_ofFn]
+  have ⟨⟨k,hk⟩,ha⟩ := ha; cases ha; simp
+  conv => rhs; change (m+1)*n + m; rw [Nat.add_comm _ m]
+  apply Nat.add_lt_add
+  . rewrite [← Nat.sub_add_eq]
+    exact m.sub_lt i.pos k.zero_lt_succ
+  . exact Nat.mul_lt_mul_of_pos_left j.2 m.zero_lt_succ
+
+theorem pivot_not_mem_pathT (i : Fin m) (j : Fin n) : Board.pivot i j ∉ Board.pathT i j := by
+  dsimp [Board.pathT, Board.pivot]; simp only [List.mem_ofFn, not_exists]
+  intro k
+  refine Fin.ne_of_val_ne (Nat.ne_of_gt ?_)
+  refine Fin.rlexProd_lt_iff.mpr (Or.inr ?_)
+  simp only [Fin.castSucc_lt_castSucc_iff, true_and]
+  show i < m-k.1-1
+  rewrite [← Nat.sub_add_eq]
+  apply Nat.lt_sub_of_add_lt
+  rewrite [← Nat.add_assoc, Nat.add_comm i.1 k.1, Nat.add_assoc]
+  exact Nat.add_lt_of_lt_sub k.2
+
+protected def path (i : Fin m) (j : Fin n) : List (Fin ((m+1)*(n+1))) :=
+  Board.pathL i j ++ Board.pathB n i ++ Board.pathR m j ++ Board.pathT i j
+
+theorem lt_last_of_mem_path (i : Fin m) (j : Fin n) (a : Fin ((m+1)*(n+1))) (ha : a ∈ Board.path i j) : a.1 < (m+1)*(n+1)-1 := by
+  conv at ha =>
+    dsimp [Board.path]
+    simp only [List.mem_append, or_assoc]
+  rcases ha with hL | hB | hR | hT
+  . exact lt_last_of_mem_pathL i j a hL
+  . exact lt_last_of_mem_pathB n i a hB
+  . exact lt_last_of_mem_pathR m j a hR
+  . exact lt_last_of_mem_pathT i j a hT
+
+theorem pivot_not_mem_path (i : Fin m) (j : Fin n) : Board.pivot i j ∉ Board.path i j := by
+  dsimp [Board.path]
+  simp only [List.mem_append, or_assoc, not_or]
+  exact ⟨
+    pivot_not_mem_pathL i j,
+    pivot_not_mem_pathB i j,
+    pivot_not_mem_pathR i j,
+    pivot_not_mem_pathT i j
+  ⟩
+
+def cycle (i : Fin m) (j : Fin n) : Permutation ((m+1)*(n+1)-1) :=
+  Permutation.cyclic <| Fin.restrict (Board.pivot i j) (pivot_lt_last i j) ::
+    (Board.path i j).pmap Fin.restrict (lt_last_of_mem_path i j)
+
+theorem sign_cycle (i : Fin m) (j : Fin n) : (cycle i j).sign = false := by
+  dsimp [cycle]
+  rewrite [Permutation.sign_cyclic_cons]
+  . simp only [List.length_pmap, beq_eq_false_iff_ne, ne_eq]
+    dsimp [Board.path, Board.pathL, Board.pathB, Board.pathR, Board.pathT]
+    simp only [List.length_append, List.length_ofFn]
+    rewrite [Nat.add_assoc (n-j.1 + (m-i.1-1)), ← Nat.mul_two, Nat.mul_mod_left]
+    decide
+  . simp only [List.mem_pmap, not_exists]
+    intro a ha hcntr
+    cases Fin.restrict_inj _ _ hcntr.2
+    exact absurd hcntr.1 <| pivot_not_mem_path i j
+
+def applyCyc (b : Board (m+1) (n+1)) (i : Fin m) (j : Fin n) (k : Int := 1) : Board (m+1) (n+1) :=
+  b.apply ((cycle i j)^k) <|
+    Permutation.sign_powInt_of_even _ k (sign_cycle i j)
+
+end Board
+
