Main.lean
@@ -1,4 +1,35 @@
 import «Fifteen»
 
+open ProofWidgets
+
+def testb : Board 4 4 where
+  val := {
+    val := #[6,8,11,1,10,5,9,3,7,2,4,13,12,14,0]
+    size_eq := by rfl
+    nodup := by rewrite [List.toArray_eq_array_mk]; decide
+  }
+  even := by rfl
+
+#html Board.toHtml {} <| (Board.solved 4 4) |>.applyCyc 0 0 8
+#html Board.toHtml {} <| testb
+  |>.applyCyc 0 2 (-2)
+  |>.applyCyc 1 1 2
+  |>.applyCyc 0 2 5
+  |>.applyCyc 1 1 5
+  |>.applyCyc 1 0 (-3)
+  |>.applyCyc 0 0
+  |>.applyCyc 2 2 (-1)
+  |>.applyCyc 0 1
+  |>.applyCyc 2 2
+  |>.applyCyc 0 2 4
+  |>.applyCyc 1 1 (-1)
+  |>.applyCyc 1 2 2
+  |>.applyCyc 2 1 2
+  |>.applyCyc 1 2 2
+  |>.applyCyc 2 2
+  |>.applyCyc 1 2 (-1)
+  |>.applyCyc 2 2
+
+
 def main : IO Unit :=
   IO.println s!"Hello, {hello}!"
